finished the first stage of the SoftBound proofs  1) SB semantics back-simulates LLVM opsem if it does not abort  2) SB opsem is not stuck because of spatial memory violation, although it can still be stuck by temporal violation or alignment failtures
The version and the last checkin added some new well-formedness rules :
  all types are well-formed --- can be allocated, and well-alignmented;
  plus, recursive types are not cyclic.

The proofs assume 1) external calls are spatial memory safe, 2)
extractValue and insertValue do nothing about pointers.



git-svn-id: https://webdav.seas.upenn.edu/svn/sol/vol@2998 eef5ea85-cc2e-0410-bd84-0fae1f012da8

src/ssa/genericvalues.v
@@ -82,118 +82,6 @@ match (GV2int TD Size.One gv) with
 | _ => false
 end.
 
-Fixpoint gen_utyp_maps_aux (cid:id) (m:list(id*typ)) (t:typ) : option typ :=
- match t with
- | typ_int s => Some (typ_int s)
- | typ_floatpoint f => Some (typ_floatpoint f)
- | typ_void => Some typ_void
- | typ_label => Some typ_label
- | typ_metadata => Some typ_metadata
- | typ_array s t0 => do ut0 <- gen_utyp_maps_aux cid m t0; ret (typ_array s ut0)
- | typ_function t0 ts0 va => 
-     do ut0 <- gen_utyp_maps_aux cid m t0;
-     do uts0 <- gen_utyps_maps_aux cid m ts0;
-        ret (typ_function ut0 uts0 va)
- | typ_struct ts0 => 
-     do uts0 <- gen_utyps_maps_aux cid m ts0; ret (typ_struct uts0)
- | typ_pointer t0 => 
-     match gen_utyp_maps_aux cid m t0 with
-     | Some ut0 => Some (typ_pointer ut0)
-     | None => 
-         match t0 with
-         | typ_namedt i => if eq_atom_dec i cid then Some t else None
-         | _ => None
-         end
-     end
- | typ_opaque => Some typ_opaque
- | typ_namedt i => lookupAL _ m i
- end
-with gen_utyps_maps_aux (cid:id) (m:list(id*typ)) (ts:list_typ) : option list_typ
-   := 
- match ts with
- | Nil_list_typ => Some Nil_list_typ
- | Cons_list_typ t0 ts0 =>
-     do ut0 <- gen_utyp_maps_aux cid m t0; 
-     do uts0 <- gen_utyps_maps_aux cid m ts0; 
-     ret (Cons_list_typ ut0 uts0)
- end.
-
-Fixpoint gen_utyp_maps (nts:namedts) : list (id*typ) :=
-match nts with
-| nil => nil 
-| namedt_intro id0 t::nts' =>
-  let results := gen_utyp_maps nts' in
-  match gen_utyp_maps_aux id0 results t with
-  | None => results
-  | Some r => (id0, r)::results
-  end
-end.
-
-Fixpoint typ2utyp_aux (m:list(id*typ)) (t:typ) : option typ :=
- match t with
- | typ_int s => Some (typ_int s)
- | typ_floatpoint f => Some (typ_floatpoint f)
- | typ_void => Some typ_void
- | typ_label => Some typ_label
- | typ_metadata => Some typ_metadata
- | typ_array s t0 => do ut0 <- typ2utyp_aux m t0; ret (typ_array s ut0)
- | typ_function t0 ts0 va => 
-     do ut0 <- typ2utyp_aux m t0;
-     do uts0 <- typs2utyps_aux m ts0;
-        ret (typ_function ut0 uts0 va)
- | typ_struct ts0 => do uts0 <- typs2utyps_aux m ts0; ret (typ_struct uts0)
- | typ_pointer t0 => do ut0 <- typ2utyp_aux m t0; ret (typ_pointer ut0)
- | typ_opaque => Some typ_opaque
- | typ_namedt i => lookupAL _ m i
- end
-with typs2utyps_aux (m:list(id*typ)) (ts:list_typ) : option list_typ := 
- match ts with
- | Nil_list_typ => Some Nil_list_typ
- | Cons_list_typ t0 ts0 =>
-     do ut0 <- typ2utyp_aux m t0; 
-     do uts0 <- typs2utyps_aux m ts0; 
-     ret (Cons_list_typ ut0 uts0)
- end.
-
-Definition typ2utyp' (nts:namedts) (t:typ) : option typ :=
-let m := gen_utyp_maps (List.rev nts) in
-typ2utyp_aux m t.
-
-Fixpoint subst_typ (i':id) (t' t:typ) : typ :=
- match t with
- | typ_int _ | typ_floatpoint _ | typ_void | typ_label | typ_metadata 
- | typ_opaque => t
- | typ_array s t0 => typ_array s (subst_typ i' t' t0)
- | typ_function t0 ts0 va => 
-     typ_function (subst_typ i' t' t0) (subst_typs i' t' ts0) va
- | typ_struct ts0 => typ_struct (subst_typs i' t' ts0)
- | typ_pointer t0 => typ_pointer (subst_typ i' t' t0)
- | typ_namedt i => if (eq_atom_dec i i') then t' else t
- end
-with subst_typs (i':id) (t':typ) (ts:list_typ) : list_typ := 
- match ts with
- | Nil_list_typ => Nil_list_typ
- | Cons_list_typ t0 ts0 =>
-     Cons_list_typ (subst_typ i' t' t0) (subst_typs i' t' ts0)
- end.
-
-Fixpoint subst_typ_by_nts (nts:namedts) (t:typ) : typ :=
-match nts with
-| nil => t
-| (namedt_intro id' t')::nts' => subst_typ_by_nts nts' (subst_typ id' t' t)
-end.
-
-Fixpoint subst_nts_by_nts (nts0 nts:namedts) : list (id*typ) :=
-match nts with
-| nil => nil
-| (namedt_intro id' t')::nts' => 
-    (id',(subst_typ_by_nts nts0 t'))::subst_nts_by_nts nts0 nts'
-end.
-
-Definition typ2utyp (nts:namedts) (t:typ) : option typ :=
-let m := subst_nts_by_nts nts nts in
-typ2utyp_aux m t.
-
 Fixpoint mgetoffset_aux (TD:TargetData) (t:typ) (idxs:list Z) (accum:Z) 
   : option Z := 
   match idxs with
@@ -220,7 +108,7 @@ Fixpoint mgetoffset_aux (TD:TargetData) (t:typ) (idxs:list Z) (accum:Z)
 
 Definition mgetoffset (TD:TargetData) (t:typ) (idxs:list Z) : option int32 := 
 let (_, nts) := TD in
-do ut <- typ2utyp nts t;
+do ut <- Constant.typ2utyp nts t;
 do z <- mgetoffset_aux TD ut idxs 0;
 ret (Int.repr 31 z).
 
@@ -1441,16 +1329,22 @@ Qed.
 *)
 
 (** allocate memory with size and alignment *)
+
 Definition malloc (TD:TargetData) (M:mem) (bsz:sz) (gn:GenericValue) (al:align) 
   : option (mem * mblock)%type :=
 match GV2int TD Size.ThirtyTwo gn with
-| Some n => Some (Mem.alloc M 0 ((Size.to_Z bsz) * n))
+| Some n => 
+    if (Coqlib.zle 0 ((Size.to_Z bsz) * n)) then
+      Some (Mem.alloc M 0 ((Size.to_Z bsz) * n))
+    else None
 | None => None
 end.
 
 Definition malloc_one (TD:TargetData) (M:mem) (bsz:sz) (al:align) 
   : option (mem * mblock)%type :=
-Some (Mem.alloc M 0 (Size.to_Z bsz)).
+if (Coqlib.zle 0 (Size.to_Z bsz)) then
+  Some (Mem.alloc M 0 (Size.to_Z bsz))
+else None.
 
 Definition free (TD:TargetData) (M:mem) (ptr:mptr) : option mem :=
 match GV2ptr TD (getPointerSize TD) ptr with
@@ -1500,6 +1394,57 @@ match GV2ptr TD (getPointerSize TD) ptr with
   end
 | _ => None
 end.
+
+Lemma free_inv : forall TD Mem0 gv Mem',
+  free TD Mem0 gv = ret Mem' ->
+  exists blk, exists ofs, exists hi, exists lo,
+    GV2ptr TD (getPointerSize TD) gv = Some (Vptr blk ofs) /\
+    Int.signed 31 ofs = 0%Z /\
+    (lo, hi) = Mem.bounds Mem0 blk /\
+    Mem.free Mem0 blk lo hi = Some Mem'.
+Proof.
+  intros TD Mem0 gv Mem' H0.
+  unfold free in H0.
+  destruct (GV2ptr TD (getPointerSize TD) gv); try solve [inversion H0; subst].
+  destruct v; try solve [inversion H0; subst].
+  destruct (Coqlib.zeq (Int.signed 31 i0) 0); try solve [inversion H0; subst].
+  remember (Mem.bounds Mem0 b) as R.
+  destruct R as [l h].
+  exists b. exists i0. rewrite e. rewrite <- HeqR. exists h. exists l.
+  repeat (split; auto).
+Qed.  
+
+Lemma malloc_inv : forall TD Mem0 tsz gn align0 Mem' mb,
+  malloc TD Mem0 tsz gn align0 = ret (Mem', mb) ->
+  exists n, GV2int TD Size.ThirtyTwo gn = Some n /\
+    (0 <= (Size.to_Z tsz) * n)%Z /\
+    Mem.alloc Mem0 0 (Size.to_Z tsz * n) = (Mem', mb).
+Proof.
+  intros.
+  unfold malloc in H.
+  destruct (GV2int TD Size.ThirtyTwo gn); try solve [inversion H; subst].
+  destruct (Coqlib.zle 0 (Size.to_Z tsz * z)); inversion H; subst.
+  exists z.
+  destruct (Mem.alloc Mem0 0 (Size.to_Z tsz * z)).
+  repeat (split; auto).
+Qed.
+
+Lemma store_inv : forall TD Mem0 gvp t gv align Mem',
+  mstore TD Mem0 gvp t gv align = Some Mem' ->
+  exists b, exists ofs, exists c, exists v0,
+    GV2ptr TD (getPointerSize TD) gvp = Some (Vptr b ofs) /\
+    typ2memory_chunk t = Some c /\
+    GV2val TD gv = Some v0 /\
+    Mem.store c Mem0 b (Int.signed 31 ofs) v0 = Some Mem'.
+Proof.
+  intros TD Mem0 gvp t gv align Mem' H.
+  unfold mstore in H.
+  destruct (GV2ptr TD (getPointerSize TD) gvp); try solve [inversion H; subst].
+  destruct v; try solve [inversion H; subst].
+  destruct (typ2memory_chunk t); try solve [inversion H; subst].
+  destruct (GV2val TD gv); try solve [inversion H; subst].
+  exists b. exists i0. exists m. exists v. split; auto.
+Qed.
 
 End LLVMgv.
 
