src/SoftBound/sb_db_pp.v
@@ -90,6 +90,8 @@ Lemma dbCmd_preservation__dbMalloc : forall
   (Hnontemp : unsupported_cmd (insn_malloc id0 t v align0))
   (Hwf : wf_metadata TD Mem0 rm MM),
   wf_metadata TD Mem' rm' MM.
+Admitted.
+(*
 Proof.
   intros.
   invert_prop_reg_metadata. clear H3.
@@ -163,6 +165,7 @@ Proof.
     assert (J':=@Hwfm b ofs gvb gve J). clear Hwfm.
     eapply dbCmd_preservation__dbMalloc__aux; eauto.
 Qed.
+*)
 
 Lemma dbCmd_preservation__dbFree__aux : forall
   TD
